Add HTLgen

src/translation/HTLgen.v
@@ -16,8 +16,344 @@
  * along with this program.  If not, see <https://www.gnu.org/licenses/>.
  *)
 
-From coqup Require Import HTL Coquplib.
 From compcert Require Import Maps.
 From compcert Require Errors.
 From compcert Require Import AST RTL.
+From coqup Require Import Verilog HTL Coquplib AssocMap Value Statemonad.
 
+Hint Resolve AssocMap.gempty : htlh.
+Hint Resolve AssocMap.gso : htlh.
+Hint Resolve AssocMap.gss : htlh.
+Hint Resolve Ple_refl : htlh.
+Hint Resolve Ple_succ : htlh.
+
+Record state: Type := mkstate {
+  st_st : reg;
+  st_freshreg: reg;
+  st_freshstate: node;
+  st_datapath: datapath;
+  st_controllogic: controllogic;
+}.
+
+Definition init_state (st : reg) : state :=
+  mkstate st
+          1%positive
+          1%positive
+          (AssocMap.empty stmnt)
+          (AssocMap.empty stmnt).
+
+Module HTLState <: State.
+
+  Definition st := state.
+
+  Inductive st_incr: state -> state -> Prop :=
+    state_incr_intro:
+      forall (s1 s2: state),
+        st_st s1 = st_st s2 ->
+        Ple s1.(st_freshreg) s2.(st_freshreg) ->
+        Ple s1.(st_freshstate) s2.(st_freshstate) ->
+        (forall n,
+            s1.(st_datapath)!n = None \/ s2.(st_datapath)!n = s1.(st_datapath)!n) ->
+        (forall n,
+            s1.(st_controllogic)!n = None
+            \/ s2.(st_controllogic)!n = s1.(st_controllogic)!n) ->
+        st_incr s1 s2.
+  Hint Constructors st_incr : htlh.
+
+  Definition st_prop := st_incr.
+  Hint Unfold st_prop : htlh.
+
+  Lemma st_refl : forall s, st_prop s s.
+  Proof. auto with htlh. Qed.
+
+  Lemma st_trans :
+    forall s1 s2 s3, st_prop s1 s2 -> st_prop s2 s3 -> st_prop s1 s3.
+  Proof.
+    intros. inv H. inv H0. apply state_incr_intro; eauto using Ple_trans.
+    - rewrite H1. rewrite H. reflexivity.
+    - intros. destruct H4 with n.
+      + left; assumption.
+      + destruct H8 with n;
+          [ rewrite <- H0; left; assumption
+          | right; rewrite <- H0; apply H10
+          ].
+    - intros. destruct H5 with n.
+      + left; assumption.
+      + destruct H9 with n.
+        * rewrite <- H0. left. assumption.
+        * right. rewrite <- H0. apply H10.
+  Qed.
+
+End HTLState.
+Import HTLState.
+
+Module HTLMonad := Statemonad(HTLState).
+Import HTLMonad.
+
+Module HTLMonadExtra := Monad.MonadExtra(HTLMonad).
+Import HTLMonadExtra.
+Import MonadNotation.
+
+Definition state_goto (st : reg) (n : node) : stmnt :=
+  Vnonblock (Vvar st) (Vlit (posToValue 32 n)).
+
+Definition state_cond (st : reg) (c : expr) (n1 n2 : node) : stmnt :=
+  Vnonblock (Vvar st) (Vternary c (posToExpr 32 n1) (posToExpr 32 n2)).
+
+Definition check_empty_node_datapath:
+  forall (s: state) (n: node), { s.(st_datapath)!n = None } + { True }.
+Proof.
+  intros. case (s.(st_datapath)!n); intros. right; auto. left; auto.
+Defined.
+
+Definition check_empty_node_controllogic:
+  forall (s: state) (n: node), { s.(st_controllogic)!n = None } + { True }.
+Proof.
+  intros. case (s.(st_controllogic)!n); intros. right; auto. left; auto.
+Defined.
+
+Lemma add_instr_state_incr :
+  forall s n n' st,
+    (st_datapath s)!n = None ->
+    (st_controllogic s)!n = None ->
+    st_incr s
+    (mkstate
+       s.(st_st)
+       s.(st_freshreg)
+       (st_freshstate s)
+       (AssocMap.add n st s.(st_datapath))
+       (AssocMap.add n (state_goto s.(st_st) n') s.(st_controllogic))).
+Proof.
+  constructor; intros;
+    try (simpl; destruct (peq n n0); subst);
+    auto with htlh.
+Qed.
+
+Definition add_instr (n : node) (n' : node) (st : stmnt) : mon unit :=
+  fun s =>
+    match check_empty_node_datapath s n, check_empty_node_controllogic s n with
+    | left STM, left TRANS =>
+      OK tt (mkstate
+               s.(st_st)
+               s.(st_freshreg)
+               (st_freshstate s)
+               (AssocMap.add n st s.(st_datapath))
+               (AssocMap.add n (state_goto s.(st_st) n') s.(st_controllogic)))
+         (add_instr_state_incr s n n' st STM TRANS)
+    | _, _ => Error (Errors.msg "HTL.add_instr")
+    end.
+
+Definition nonblock (dst : reg) (e : expr) := Vnonblock (Vvar dst) e.
+Definition block (dst : reg) (e : expr) := Vblock (Vvar dst) e.
+
+Definition bop (op : binop) (r1 r2 : reg) : expr :=
+  Vbinop op (Vvar r1) (Vvar r2).
+
+Definition boplit (op : binop) (r : reg) (l : Integers.int) : expr :=
+  Vbinop op (Vvar r) (Vlit (intToValue l)).
+
+Definition boplitz (op: binop) (r: reg) (l: Z) : expr :=
+  Vbinop op (Vvar r) (Vlit (ZToValue 32%nat l)).
+
+Definition translate_comparison (c : Integers.comparison) (args : list reg) : mon expr :=
+  match c, args with
+  | Integers.Ceq, r1::r2::nil => ret (bop Veq r1 r2)
+  | Integers.Cne, r1::r2::nil => ret (bop Vne r1 r2)
+  | Integers.Clt, r1::r2::nil => ret (bop Vlt r1 r2)
+  | Integers.Cgt, r1::r2::nil => ret (bop Vgt r1 r2)
+  | Integers.Cle, r1::r2::nil => ret (bop Vle r1 r2)
+  | Integers.Cge, r1::r2::nil => ret (bop Vge r1 r2)
+  | _, _ => error (Errors.msg "Veriloggen: comparison instruction not implemented: other")
+  end.
+
+Definition translate_comparison_imm (c : Integers.comparison) (args : list reg) (i: Integers.int)
+  : mon expr :=
+  match c, args with
+  | Integers.Ceq, r1::nil => ret (boplit Veq r1 i)
+  | Integers.Cne, r1::nil => ret (boplit Vne r1 i)
+  | Integers.Clt, r1::nil => ret (boplit Vlt r1 i)
+  | Integers.Cgt, r1::nil => ret (boplit Vgt r1 i)
+  | Integers.Cle, r1::nil => ret (boplit Vle r1 i)
+  | Integers.Cge, r1::nil => ret (boplit Vge r1 i)
+  | _, _ => error (Errors.msg "Veriloggen: comparison_imm instruction not implemented: other")
+  end.
+
+Definition translate_condition (c : Op.condition) (args : list reg) : mon expr :=
+  match c, args with
+  | Op.Ccomp c, _ => translate_comparison c args
+  | Op.Ccompu c, _ => translate_comparison c args
+  | Op.Ccompimm c i, _ => translate_comparison_imm c args i
+  | Op.Ccompuimm c i, _ => translate_comparison_imm c args i
+  | Op.Cmaskzero n, _ => error (Errors.msg "Veriloggen: condition instruction not implemented: Cmaskzero")
+  | Op.Cmasknotzero n, _ => error (Errors.msg "Veriloggen: condition instruction not implemented: Cmasknotzero")
+  | _, _ => error (Errors.msg "Veriloggen: condition instruction not implemented: other")
+  end.
+
+Definition translate_eff_addressing (a: Op.addressing) (args: list reg) : mon expr :=
+  match a, args with
+  | Op.Aindexed off, r1::nil => ret (boplitz Vadd r1 off)
+  | Op.Aindexed2 off, r1::r2::nil => ret (Vbinop Vadd (Vvar r1) (boplitz Vadd r2 off))
+  | Op.Ascaled scale offset, r1::nil =>
+    ret (Vbinop Vadd (boplitz Vadd r1 scale) (Vlit (ZToValue 32%nat offset)))
+  | Op.Aindexed2scaled scale offset, r1::r2::nil =>
+    ret (Vbinop Vadd (boplitz Vadd r1 offset) (boplitz Vmul r2 scale))
+  | _, _ => error (Errors.msg "Veriloggen: eff_addressing instruction not implemented: other")
+  end.
+
+(** Translate an instruction to a statement. *)
+Definition translate_instr (op : Op.operation) (args : list reg) : mon expr :=
+  match op, args with
+  | Op.Omove, r::nil => ret (Vvar r)
+  | Op.Ointconst n, _ => ret (Vlit (intToValue n))
+  | Op.Oneg, r::nil => ret (Vunop Vneg (Vvar r))
+  | Op.Osub, r1::r2::nil => ret (bop Vsub r1 r2)
+  | Op.Omul, r1::r2::nil => ret (bop Vmul r1 r2)
+  | Op.Omulimm n, r::nil => ret (boplit Vmul r n)
+  | Op.Omulhs, _ => error (Errors.msg "Veriloggen: Instruction not implemented: Omulhs")
+  | Op.Omulhu, _ => error (Errors.msg "Veriloggen: Instruction not implemented: Omulhu")
+  | Op.Odiv, r1::r2::nil => ret (bop Vdiv r1 r2)
+  | Op.Odivu, r1::r2::nil => ret (bop Vdivu r1 r2)
+  | Op.Omod, r1::r2::nil => ret (bop Vmod r1 r2)
+  | Op.Omodu, r1::r2::nil => ret (bop Vmodu r1 r2)
+  | Op.Oand, r1::r2::nil => ret (bop Vand r1 r2)
+  | Op.Oandimm n, r::nil => ret (boplit Vand r n)
+  | Op.Oor, r1::r2::nil => ret (bop Vor r1 r2)
+  | Op.Oorimm n, r::nil => ret (boplit Vor r n)
+  | Op.Oxor, r1::r2::nil => ret (bop Vxor r1 r2)
+  | Op.Oxorimm n, r::nil => ret (boplit Vxor r n)
+  | Op.Onot, r::nil => ret (Vunop Vnot (Vvar r))
+  | Op.Oshl, r1::r2::nil => ret (bop Vshl r1 r2)
+  | Op.Oshlimm n, r::nil => ret (boplit Vshl r n)
+  | Op.Oshr, r1::r2::nil => ret (bop Vshr r1 r2)
+  | Op.Oshrimm n, r::nil => ret (boplit Vshr r n)
+  | Op.Oshrximm n, r::nil => error (Errors.msg "Veriloggen: Instruction not implemented: Oshrximm")
+  | Op.Oshru, r1::r2::nil => error (Errors.msg "Veriloggen: Instruction not implemented: Oshru")
+  | Op.Oshruimm n, r::nil => error (Errors.msg "Veriloggen: Instruction not implemented: Oshruimm")
+  | Op.Ororimm n, r::nil => error (Errors.msg "Veriloggen: Instruction not implemented: Ororimm")
+  | Op.Oshldimm n, r::nil => error (Errors.msg "Veriloggen: Instruction not implemented: Oshldimm")
+  | Op.Ocmp c, _ => translate_condition c args
+  | Op.Olea a, _ => translate_eff_addressing a args
+  | _, _ => error (Errors.msg "Veriloggen: Instruction not implemented: other")
+  end.
+
+Lemma add_branch_instr_state_incr:
+  forall s e n n1 n2,
+    (st_datapath s) ! n = None ->
+    (st_controllogic s) ! n = None ->
+    st_incr s (mkstate
+                 s.(st_st)
+                (st_freshreg s)
+                (st_freshstate s)
+                (AssocMap.add n Vskip (st_datapath s))
+                (AssocMap.add n (state_cond s.(st_st) e n1 n2) (st_controllogic s))).
+Proof.
+  intros. apply state_incr_intro; simpl;
+            try (intros; destruct (peq n0 n); subst);
+            auto with htlh.
+Qed.
+
+Definition add_branch_instr (e: expr) (n n1 n2: node) : mon unit :=
+  fun s =>
+    match check_empty_node_datapath s n, check_empty_node_controllogic s n with
+    | left NSTM, left NTRANS =>
+      OK tt (mkstate
+               s.(st_st)
+                (st_freshreg s)
+                (st_freshstate s)
+                (AssocMap.add n Vskip (st_datapath s))
+                (AssocMap.add n (state_cond s.(st_st) e n1 n2) (st_controllogic s)))
+         (add_branch_instr_state_incr s e n n1 n2 NSTM NTRANS)
+    | _, _ => Error (Errors.msg "Veriloggen: add_branch_instr")
+    end.
+
+Definition transf_instr (fin rtrn: reg) (ni: node * instruction) : mon unit :=
+  match ni with
+    (n, i) =>
+    match i with
+    | Inop n' => add_instr n n' Vskip
+    | Iop op args dst n' =>
+      do instr <- translate_instr op args;
+      add_instr n n' (block dst instr)
+    | Iload _ _ _ _ _ => error (Errors.msg "Loads are not implemented.")
+    | Istore _ _ _ _ _ => error (Errors.msg "Stores are not implemented.")
+    | Icall _ _ _ _ _ => error (Errors.msg "Calls are not implemented.")
+    | Itailcall _ _ _ => error (Errors.msg "Tailcalls are not implemented.")
+    | Ibuiltin _ _ _ _ => error (Errors.msg "Builtin functions not implemented.")
+    | Icond cond args n1 n2 =>
+      do e <- translate_condition cond args;
+      add_branch_instr e n n1 n2
+    | Ijumptable _ _ => error (Errors.msg "Jumptable not implemented")
+    | Ireturn r =>
+      match r with
+      | Some r' =>
+        add_instr n n (Vseq (block fin (Vlit (ZToValue 1%nat 1%Z))) (block rtrn (Vvar r')))
+      | None =>
+        add_instr n n (block fin (Vlit (ZToValue 1%nat 1%Z)))
+      end
+    end
+  end.
+
+Lemma create_reg_state_incr:
+  forall s,
+    st_incr s (mkstate
+         s.(st_st)
+         (Pos.succ (st_freshreg s))
+         (st_freshstate s)
+         (st_datapath s)
+         (st_controllogic s)).
+Proof. constructor; simpl; auto with htlh. Qed.
+
+Definition create_reg: mon reg :=
+  fun s => let r := s.(st_freshreg) in
+           OK r (mkstate
+                   s.(st_st)
+                   (Pos.succ r)
+                   (st_freshstate s)
+                   (st_datapath s)
+                   (st_controllogic s))
+              (create_reg_state_incr s).
+
+Definition transf_module (f: function) : mon module :=
+  do fin <- create_reg;
+  do rtrn <- create_reg;
+  do _ <- traverselist (transf_instr fin rtrn) (Maps.PTree.elements f.(RTL.fn_code));
+  do start <- create_reg;
+  do rst <- create_reg;
+  do clk <- create_reg;
+  do current_state <- get;
+  ret (mkmodule
+         f.(RTL.fn_params)
+         current_state.(st_datapath)
+         current_state.(st_controllogic)
+         f.(fn_entrypoint)
+         current_state.(st_st)
+         fin
+         rtrn).
+
+Definition max_state (f: function) : state :=
+  let st := Pos.succ (max_reg_function f) in
+  mkstate st
+          (Pos.succ st)
+          (Pos.succ (max_pc_function f))
+          (st_datapath (init_state st))
+          (st_controllogic (init_state st)).
+
+Definition transl_module (f : function) : Errors.res module :=
+  run_mon (max_state f) (transf_module f).
+
+Fixpoint main_function (main : ident) (flist : list (ident * AST.globdef fundef unit))
+{struct flist} : option function :=
+  match flist with
+  | (i, AST.Gfun (AST.Internal f)) :: xs =>
+    if Pos.eqb i main
+    then Some f
+    else main_function main xs
+  | _ :: xs => main_function main xs
+  | nil => None
+  end.
+
+Definition transf_program (d : program) : Errors.res module :=
+  match main_function d.(AST.prog_main) d.(AST.prog_defs) with
+  | Some f => run_mon (max_state f) (transf_module f)
+  | _ => Errors.Error (Errors.msg "HTL: could not find main function")
+  end.
